Finish proof of normalization preserving semantics

src/GraphAux.v
@@ -8,83 +8,96 @@ From extructures Require Import ord fset fmap.
 Require Import Graph.
 
 
+
 Section GraphAux.
 
   Variables (F Vals : ordType).
-  Implicit Type graph :  @graphQLGraph F Vals.
+  Variable (graph :  @graphQLGraph F Vals).
   Implicit Type edge : @node F Vals * @fld F Vals * @node F Vals.
+
   
+  Open Scope fset.
 
   (** Extractors for an edge **)
-  Definition edge_nodes edge : seq node :=
-    let: (u, _, v) := edge in [:: u ; v].
 
-  Definition edge_target edge : node :=
+
+  Definition etarget edge : node :=
     let: (_, _, v) := edge in v.
 
-  Definition edge_source edge : node :=
+  Definition esource edge : node :=
     let: (u, _, _) := edge in u.
 
-  Definition edge_field edge : fld :=
+  Definition efield edge : fld :=
     let: (_, f, _) := edge in f.
 
+  Definition enodes edge : seq node := [:: edge.(esource) ; edge.(etarget)].
   
   (** Get all nodes from a graph **)
-  Definition nodes graph : {fset node} :=
-    fset (graph.(root) :: (flatten [seq (edge_nodes edge) | edge <- graph.(E)])).
+  Definition nodes graph : seq node :=
+    undup (graph.(root) ::  flatten [seq edge.(enodes) | edge <- graph.(E)]).
 
 
-  Lemma root_in_nodes graph : graph.(root) \in nodes graph.
+  Lemma in_undup {A : eqType} (s : seq A) (x : A) :
+    x \in s <-> x \in undup s.
   Proof.
-    rewrite /nodes.
-    rewrite in_fset inE. 
-    by apply/orP; left; apply/eqP.
+    elim: s => //= y s [IHl IHr]; split.
+    - rewrite inE => /orP [/eqP <- | Hin]; case: ifP => //=.
+      * by intros; apply/orP; left; apply/eqP.
+      * by intros; apply: IHl.
+      * by intros; apply/orP; right; apply: IHl.
+    - case: ifP => //=; intros; rewrite inE; apply/orP.
+      * by right; apply: IHr.
+      * by case/orP: H => [/eqP <- | Hin]; [left; apply/eqP | right; apply: IHr].      
+  Qed.
+    
+  Lemma root_in_nodes : graph.(root) \in graph.(nodes).
+  Proof.
+    rewrite /nodes -in_undup.
+      by apply/orP; left; apply/eqP.
   Qed.
 
 
   (** Get all neighbours of a node irrespective of the field in the edge 
       connecting the two **)
-  Definition neighbours graph (u : node) : seq node :=
-    undup (foldr (fun e acc =>
-                   let: (u', _, v) := e in
-                   if u' == u then
-                     v :: acc
-                   else
-                     acc) [::] graph.(E)).
+  Definition neighbours (u : node) (edges : seq (node * fld * node)) : seq node :=
+    undup [seq edge.(etarget) | edge <- edges & edge.(esource) == u]. 
+
   
-  (* fset [seq (edge_target edge) | edge <- [seq edge <- graph.(E) | edge_source edge == u]]. *)
 
 
   (** Get all neighbours of a node that are linked via an edge with a given
       field. **)
-  Definition neighbours_with_field graph (u : node) (f : fld) : seq node :=
-    undup [seq (edge_target edge) |  edge <- graph.(E) & ((edge_source edge == u) && (edge_field edge == f))].
+  Definition neighbours_with_field (u : node) (f : fld) : seq node :=
+    undup [seq edge.(etarget) |  edge <- [seq edge <- graph.(E) | (esource edge == u) & (efield edge == f)]].
 
 
   (** 
       Checks whether there is only one edge coming out of the source node and 
       having the given field.
    **)
-  Definition is_field_unique_for_src_node graph (src_node : node) (f : fld) :=
-    let edges :=
-        [seq edge <- graph.(E) | (edge_source edge == src_node) & (edge_field edge == f)]
-    in
-    uniq edges.
+  Definition is_field_unique_for_src_node graph (src_node : node) (f : fld) : bool :=
+    uniq [seq edge <- graph.(E) | (esource edge == src_node) & (efield edge == f)].
 
 
+    
+ 
   
-
-  
-  
-  Lemma u_and_target_nodes_in_nodes graph u fld :
-    u \in graph.(nodes) -> all (fun v => v \in graph.(nodes)) (neighbours_with_field graph u fld).
+  Lemma neighbours_are_in_nodes u fld:
+    forall x, x \in neighbours_with_field u fld -> x \in graph.(nodes).
   Proof.
-  Admitted.
-
-  
+    rewrite /neighbours_with_field /nodes => x.
+    rewrite -?in_undup => /mapP [v].
+    rewrite mem_filter => /andP [/andP [/eqP Hsrc /eqP Hfld] Hin] /= Heq.
+    apply/orP; right.
+    apply/flatten_mapP.
+    exists v => //=.
+    rewrite /enodes inE; apply/orP; right.
+    by rewrite mem_seq1; apply/eqP.
+  Qed.
+   
   
     
-  Lemma ohead_in_nodes graph nds v :
+  Lemma ohead_in_nodes nds v :
     all (fun node => node \in graph.(nodes)) nds ->
     ohead nds = Some v ->
     v \in graph.(nodes). 
